HOL_To_IMP_Minus/Refinements/HOL_To_IMP_Minus_Fun_Pattern_Setup.thy
@@ -1,0 +1,48 @@
+\<^marker>\<open>creator "Kevin Kappelmann"\<close>
+theory HOL_To_IMP_Minus_Fun_Pattern_Setup
+  imports
+    HOL_To_IMP_Minus_Primitives
+    "HOL-Library.Simps_Case_Conv"
+begin
+
+context HOL_To_IMP_Minus
+begin
+
+lemma case_nat_eq_if: "(case n of 0 \<Rightarrow> x | Suc x \<Rightarrow> f x) = (if n = 0 then x else f (n - 1))"
+  unfolding Nitpick.case_nat_unfold by simp
+
+end
+
+paragraph \<open>Example application:\<close>
+
+experiment
+begin
+
+interpretation HOL_To_IMP_Minus .
+
+fun add_nat_pat :: "nat \<Rightarrow> nat \<Rightarrow> nat \<Rightarrow> nat" where
+"add_nat_pat 0 0 z = z" |
+"add_nat_pat 0 (Suc y) z = add_nat_pat 0 y (z + 1)" |
+"add_nat_pat (Suc x) y z = add_nat_pat x y (z + 1)"
+declare add_nat_pat.simps[simp del]
+                        
+case_of_simps add_nat_pat_eq[simplified Nitpick.case_nat_unfold] : add_nat_pat.simps
+compile_nat add_nat_pat_eq basename add_pat
+
+lemma add_nat_pat_IMP_func_correct:
+  assumes "(tailcall_to_IMP_Minus add_pat_IMP, s) \<Rightarrow>\<^bsup>t\<^esup> s'"
+  shows "s' ''add_pat_ret'' = add_nat_pat (s ''add_pat_x1a'') (s ''add_pat_x2a'') (s ''add_pat_x3ba'')"
+  using assms                                 
+  apply (rule tailcall_to_IMP_Minus_correct_if_correct)
+  apply (subst compiled_const_defs, simp)
+  apply (subst compiled_const_defs, simp)
+  subgoal for t s'
+  apply (induction "(s ''add_pat_x1a'')" "(s ''add_pat_x2a'')" "(s ''add_pat_x3ba'')" arbitrary: s t rule: add_nat_pat.induct)
+  apply (tactic \<open>H.start_run_finish_pattern_fun_tac @{thms compiled_const_defs} @{thms func_correct} 
+    @{thms add_nat_pat.simps} @{context} 1\<close>)+
+  done
+  done
+
+end
+
+end
